src/cbor/pulse/CBOR.Pulse.API.Det.Common.fsti
@@ -258,6 +258,10 @@ val cbor_det_array_iterator_next () : array_iterator_next_t cbor_det_match cbor_
 
 val cbor_det_array_iterator_truncate () : array_iterator_truncate_t cbor_det_array_iterator_match
 
+val cbor_det_array_iterator_share () : array_iterator_share_t cbor_det_array_iterator_match
+
+val cbor_det_array_iterator_gather () : array_iterator_gather_t cbor_det_array_iterator_match
+
 val cbor_det_get_array_item () : get_array_item_t cbor_det_match
 
 val cbor_det_get_map_length () : get_map_length_t cbor_det_match
