src/cbor/pulse/raw/CBOR.Pulse.Raw.Format.Serialized.fsti
@@ -71,6 +71,10 @@ val cbor_serialized_array_iterator_next (_: squash SZ.fits_u64) : cbor_raw_seria
 
 val cbor_serialized_array_iterator_truncate : cbor_raw_serialized_iterator_truncate_t cbor_serialized_array_iterator_match
 
+val cbor_serialized_array_iterator_share : cbor_raw_serialized_iterator_share_t cbor_serialized_array_iterator_match
+
+val cbor_serialized_array_iterator_gather : cbor_raw_serialized_iterator_gather_t cbor_serialized_array_iterator_match
+
 val cbor_serialized_map_iterator_match
   (p: perm)
   (i: cbor_raw_serialized_iterator)
